src/Bedrock/MakeListLengths.v
@@ -1,0 +1,59 @@
+Require Import Coq.ZArith.ZArith.
+Require Import Coq.Lists.List.
+Require Import Crypto.AbstractInterpretation.AbstractInterpretation.
+Require Import Crypto.Bedrock.Types.
+Require Import Crypto.Language.API.
+Require Import Crypto.Util.Option.
+
+Import Language.API.Compilers AbstractInterpretation.Compilers.
+Import Types Types.Notations.
+Existing Instances rep.Z rep.listZ_mem.
+
+Section with_parameters.
+  Context {p : Types.parameters}.
+
+  Fixpoint list_lengths_repeat_base (n : nat) t : base_listonly nat t :=
+    match t as t0 return base_listonly nat t0 with
+    | base.type.prod a b =>
+      (list_lengths_repeat_base n a, list_lengths_repeat_base n b)
+    | base_listZ => n
+    | _ => tt
+    end.
+  Fixpoint list_lengths_repeat_args (n : nat) t
+    : type.for_each_lhs_of_arrow list_lengths t :=
+    match t as t0 return type.for_each_lhs_of_arrow list_lengths t0 with
+    | type.base b => tt
+    | type.arrow (type.base s) d =>
+      (list_lengths_repeat_base n s, list_lengths_repeat_args n d)
+    | type.arrow s d => (tt, list_lengths_repeat_args n d)
+    end.
+
+  (* mostly a duplicate of list_lengths_from_value, just with ZRange interp *)
+  Fixpoint list_lengths_from_bounds {t}
+    : ZRange.type.base.option.interp t -> option (base_listonly nat t) :=
+    match t as t0 return
+          ZRange.type.base.option.interp t0 -> option (base_listonly nat t0) with
+    | base.type.prod a b =>
+      fun x =>
+        (x1 <- list_lengths_from_bounds (fst x);
+           x2 <- list_lengths_from_bounds (snd x);
+           Some (x1, x2))%option
+    | base_listZ =>
+      fun x : option (list _) => option_map (@List.length _) x
+    | _ => fun _ => Some tt
+    end.
+  Fixpoint list_lengths_from_argbounds {t}
+    : type.for_each_lhs_of_arrow ZRange.type.option.interp t ->
+      option (type.for_each_lhs_of_arrow list_lengths t) :=
+    match t as t0 return
+          type.for_each_lhs_of_arrow _ t0 ->
+          option (type.for_each_lhs_of_arrow _ t0) with
+    | type.base b => fun _ => Some tt
+    | type.arrow (type.base a) b =>
+      fun x =>
+        (x1 <- list_lengths_from_bounds (fst x);
+           x2 <- list_lengths_from_argbounds (snd x);
+           Some (x1, x2))%option
+    | type.arrow a b => fun _ => None
+    end.
+End with_parameters.
