src/Bedrock/VarnameGenerator.v
@@ -1,0 +1,100 @@
+Require Import Coq.ZArith.ZArith.
+Require Import Coq.Strings.String.
+Require Import Crypto.Util.Strings.Decimal.
+Require Import Crypto.Util.Tactics.BreakMatch.
+Require Import Crypto.Util.Strings.String.
+Local Open Scope string_scope.
+
+(* TODO: move this? *)
+Lemma append_eq_r_iff s1 s2 s3 :
+  s1 ++ s2 = s1 ++ s3 <-> s2 = s3.
+Proof.
+  induction s1; cbn [append]; split;
+    try inversion 1; intros; auto; [ ].
+  apply IHs1. auto.
+Qed.
+
+(* TODO: move this? *)
+Lemma append_eq_prefix :
+  forall s1 s2 s3 s4,
+    s1 ++ s2 = s3 ++ s4 ->
+    prefix s1 s3 = true \/ prefix s3 s1 = true.
+Proof.
+  induction s1; destruct s3; cbn [append prefix] in *;
+    intros; try tauto; [ ].
+  match goal with H : String _ _ = String _ _ |- _ =>
+                  inversion H; clear H; subst end.
+  break_match; subst; try tauto.
+  eapply IHs1; eauto.
+Qed.
+
+Section prefix_generator.
+  Context (pre : string).
+
+  Definition prefix_name_gen (x : nat) : string :=
+    pre ++ Z.to_string (Z.of_nat x).
+
+  Lemma prefix_name_gen_unique i j :
+    prefix_name_gen i = prefix_name_gen j <-> i = j.
+  Proof.
+    intros.
+    pose proof (Decimal.Z.of_to (Z.of_nat i)).
+    pose proof (Decimal.Z.of_to (Z.of_nat j)).
+    split; intros; [ | subst; reflexivity ].
+    match goal with H : _ |- _ => apply append_eq_r_iff in H end.
+    apply Nat2Z.inj. congruence.
+  Qed.
+
+  Lemma prefix_name_gen_prefix i :
+    prefix pre (prefix_name_gen i) = true.
+  Proof.
+    apply prefix_correct.
+    cbv [prefix_name_gen]; induction pre; intros.
+    { cbn [length]. apply substring_0_0. }
+    { cbn. congruence. }
+  Qed.
+
+  Lemma prefix_name_gen_startswith v i :
+    v = prefix_name_gen i ->
+    startswith pre v = true.
+  Proof.
+    intros; subst. cbv [startswith].
+    apply eqb_eq. symmetry. apply prefix_correct.
+    apply prefix_name_gen_prefix.
+  Qed.
+End prefix_generator.
+
+Section disjoint.
+  Definition disjoint (gen1 gen2 : nat -> string) : Prop :=
+    forall n m, gen1 n <> gen2 m.
+
+  Lemma prefix_generator_disjoint pre1 pre2 :
+    prefix pre1 pre2 = false ->
+    prefix pre2 pre1 = false ->
+    disjoint (prefix_name_gen pre1) (prefix_name_gen pre2).
+  Proof.
+    cbv [disjoint prefix_name_gen]; intros.
+    let H := fresh in
+    intro H; apply append_eq_prefix in H; destruct H;
+      congruence.
+  Qed.
+End disjoint.
+
+Section defaults.
+  Definition default_inname_gen : nat -> string :=
+    prefix_name_gen "in".
+  Definition default_outname_gen : nat -> string :=
+    prefix_name_gen "out".
+  Definition default_varname_gen : nat -> string :=
+    prefix_name_gen "x".
+
+  Lemma outname_gen_inname_gen_disjoint :
+    disjoint default_outname_gen default_inname_gen.
+  Proof. apply prefix_generator_disjoint; reflexivity. Qed.
+  Lemma inname_gen_varname_gen_disjoint :
+    disjoint default_inname_gen default_varname_gen.
+  Proof. apply prefix_generator_disjoint; reflexivity. Qed.
+  Lemma outname_gen_varname_gen_disjoint :
+    disjoint default_outname_gen default_varname_gen.
+  Proof. apply prefix_generator_disjoint; reflexivity. Qed.
+End defaults.
